Carrier/SKAT_Eval.thy
@@ -4,14 +4,6 @@ begin
 
 type_synonym 'a mems = "(nat \<Rightarrow> 'a) set"
 
-(* Non-deterministic memory forms and idempotent commutative monoid *)
-
-primrec iter :: "nat \<Rightarrow> ('a \<Rightarrow> 'a) \<Rightarrow> 'a \<Rightarrow> 'a" where
-  "iter 0 f = id"
-| "iter (Suc n) f = f \<circ> iter n f"
-
-value eval_wf_pred
-
 fun eval_bexpr ::
   "('a::ranked_alphabet, 'b) interp \<Rightarrow> 'a wf_pred bexpr \<Rightarrow> (nat \<Rightarrow> 'b) \<Rightarrow> bool"
   where
@@ -25,15 +17,13 @@ fun eval_bexpr ::
 definition filter_set :: "('a \<Rightarrow> bool) \<Rightarrow> 'a set \<Rightarrow> 'a set" where
   "filter_set p X \<equiv> \<Union>x\<in>X. if p x then {x} else {}"
 
-abbreviation set_mem where "set_mem \<equiv> setMem"
-
 definition set_mems :: "nat \<Rightarrow> ('a mem \<Rightarrow> 'a) \<Rightarrow> 'a mems \<Rightarrow> 'a mems" where
   "set_mems x f \<Delta> \<equiv> (\<lambda>mem. set_mem x (f mem) mem) ` \<Delta>"
 
-definition assigns ::
-  "('a::ranked_alphabet, 'b) interp \<Rightarrow> nat \<Rightarrow> 'a trm \<Rightarrow> 'b mems \<Rightarrow> 'b mems"
+definition wf_assigns ::
+  "('a::ranked_alphabet, 'b) interp \<Rightarrow> nat \<Rightarrow> 'a wf_trm \<Rightarrow> 'b mems \<Rightarrow> 'b mems"
   where
-  "assigns D x s mems = set_mems x (\<lambda>mem. eval_trm D mem s) mems"
+  "wf_assigns D x s mems = set_mems x (\<lambda>mem. eval_wf_trm D mem s) mems"
 
 lemma finite_set_mems: assumes "finite \<Delta>" shows "finite (set_mems x f \<Delta>)"
   by (induct rule: finite_subset_induct_var[OF assms(1), of "\<Delta>"], simp_all add: set_mems_def)
@@ -41,25 +31,27 @@ lemma finite_set_mems: assumes "finite \<Delta>" shows "finite (set_mems x f \<D
 lemma card_set_mems: "finite \<Delta> \<Longrightarrow> card (set_mems X f \<Delta>) \<le> card \<Delta>"
   by (simp add: set_mems_def, smt card_image_le)
 
-lemma assign_image: "assigns D x t mems = assign D x t ` mems"
-  by (auto simp add: assigns_def set_mems_def assign_def[symmetric])
+lemma wf_assign_image: "wf_assigns D x t mems = wf_assign D x t ` mems"
+  by (auto simp add: wf_assigns_def set_mems_def wf_assign_def[symmetric])
 
-lemma eval_assigns3: "assigns D x t (assigns D x s mems) = assigns D x (trm_subst {x} s t) mems"
-proof (auto simp add: assign_image image_def)
-  fix mem assume mem_in: "mem \<in> mems"
-  show "\<exists>m\<in>mems. assign D x t (assign D x s mem) = assign D x (trm_subst {x} s t) m"
-    by (rule bexI[OF _ mem_in], simp add: eval_assign3)
-next
-  fix mem assume mem_in: "mem \<in> mems"
-  thus "\<exists>m1. (\<exists>m2\<in>mems. m1 = assign D x s m2) \<and>
-              assign D x (trm_subst {x} s t) mem = assign D x t m1"
-    by (rule_tac x = "assign D x s mem" in exI, auto simp add: eval_assign3)
-qed
+lemma eval_wf_assigns1:
+  assumes xy: "x \<noteq> y" and ys: "y \<notin> FV s"
+  shows "wf_assigns D y t (wf_assigns D x s mems) = wf_assigns D x s (wf_assigns D y (t[x|s]) mems)"
+  by (auto simp add: wf_assign_image image_def, (metis eval_wf_assign1 xy ys)+)
+
+lemma eval_wf_assigns2:
+  assumes xy: "x \<noteq> y" and xs: "x \<notin> FV s"
+  shows "wf_assigns D y t (wf_assigns D x s mems) =
+         wf_assigns D y (t[x|s]) (wf_assigns D x s mems)"
+  by (auto simp add: wf_assign_image image_def, (metis eval_wf_assign2 xy xs)+)
+
+lemma eval_wf_assigns3: "wf_assigns D x t (wf_assigns D x s mems) = wf_assigns D x (t[x|s]) mems"
+  by (auto simp add: wf_assign_image image_def, (metis eval_wf_assign3)+)
 
 fun eval_skat_expr ::
-  "('a::ranked_alphabet, 'b) interp \<Rightarrow> 'a skat_expr \<Rightarrow> 'b mem \<Rightarrow> 'b mem"
+  "('a::ranked_alphabet, 'b) interp \<Rightarrow> 'a skat_expr \<Rightarrow> 'b mems \<Rightarrow> 'b mems"
   where
-  "eval_skat_expr D (SKLeaf X s) \<Delta> = set_mems X (\<lambda>mem. eval_wf_trm D mem s) \<Delta>"
+  "eval_skat_expr D (SKLeaf x s) \<Delta> = wf_assigns D x s \<Delta>"
 | "eval_skat_expr D (SKBool P) \<Delta> = filter_set (eval_bexpr D P) \<Delta>"
 | "eval_skat_expr D (s :\<odot>: t) \<Delta> = eval_skat_expr D t (eval_skat_expr D s \<Delta>)"
 | "eval_skat_expr D (s :\<oplus>: t) \<Delta> = eval_skat_expr D s \<Delta> \<union> eval_skat_expr D t \<Delta>"
@@ -67,8 +59,18 @@ fun eval_skat_expr ::
 | "eval_skat_expr D SKOne \<Delta> = \<Delta>"
 | "eval_skat_expr D SKZero \<Delta> = {}"
 
+definition eval_power :: "('a::ranked_alphabet, 'b) interp \<Rightarrow> 'a skat_expr \<Rightarrow> nat \<Rightarrow> 'b mems \<Rightarrow> 'b mems"
+  where "eval_power D s n \<Delta> = iter n (eval_skat_expr D s) \<Delta>"
+
+lemma eval_star_power: "eval_skat_expr D (SKStar s) \<Delta> = \<Union> {y. \<exists>n. y = eval_power D s n \<Delta>}"
+  by (auto simp add: eval_power_def)
+
+lemma eval_iter1: "eval_skat_expr D s (iter n (eval_skat_expr D s) \<Delta>)
+     = iter n (eval_skat_expr D s) (eval_skat_expr D s \<Delta>)"
+  by (induct n, auto)
+
 lemma eval_mod1: "eval_skat_expr D s {} = {}"
-proof (induct s, simp_all add: update_mem_def, clarify)
+proof (induct s, simp_all add: wf_assigns_def set_mems_def, intro allI)
   fix s n assume "eval_skat_expr D s {} = {}"
   thus "iter n (eval_skat_expr D s) {} = {}"
     by (induct n, auto)
@@ -78,7 +80,7 @@ next
 qed
 
 lemma eval_mod2: "eval_skat_expr D s (\<Delta> \<union> \<Gamma>) = eval_skat_expr D s \<Delta> \<union> eval_skat_expr D s \<Gamma>"
-  apply (induct s arbitrary: \<Delta> \<Gamma>, simp_all add: update_mem_def filter_set_def)
+  apply (induct s arbitrary: \<Delta> \<Gamma>, simp_all add: wf_assigns_def set_mems_def filter_set_def)
   apply (metis image_Un)
   apply (metis Un_assoc Un_left_commute)
 proof -
@@ -110,6 +112,171 @@ proof simp
   qed
   thus "(\<Union>n. iter n (eval_skat_expr D r) a) \<union> b = b"
     by blast
+qed
+
+lemma eval_iter:
+  "iter n (eval_skat_expr D x) (eval_skat_expr D x \<Delta>) = iter (Suc n) (eval_skat_expr D x) \<Delta>"
+  by (induct n, auto)
+
+lemma eval_star_unfoldl:
+  fixes \<Delta> :: "'b mems"
+  shows "eval_skat_expr D (SKOne :\<oplus>: x :\<odot>: SKStar x :\<oplus>: SKStar x) \<Delta> = eval_skat_expr D (SKStar x) \<Delta>"
+proof auto
+  fix mem :: "'b mem" assume "mem \<in> \<Delta>"
+  thus "\<exists>n. mem \<in> iter n (eval_skat_expr D x) \<Delta>"
+    by (rule_tac x = 0 in exI, simp)
+next
+  fix mem :: "'b mem" and n
+  assume "mem \<in> iter n (eval_skat_expr D x) (eval_skat_expr D x \<Delta>)"
+  thus "\<exists>n. mem \<in> iter n (eval_skat_expr D x) \<Delta>"
+    by (rule_tac x = "Suc n" in exI, metis eval_iter)
+qed
+
+lemma eval_iso: "\<Delta> \<subseteq> \<Gamma> \<Longrightarrow> eval_skat_expr D s \<Delta> \<subseteq> eval_skat_expr D s \<Gamma>"
+  by (metis eval_mod2 subset_Un_eq)
+
+lemma iter_jp:
+  assumes f_jp: "\<And>X. f (\<Union>X) = \<Union>(f ` X)"
+  shows "iter n f (\<Union>X) = \<Union>(iter n f ` X)"
+proof (induct n arbitrary: X, simp)
+  fix n X
+  assume "\<And>X. iter n f (\<Union>X) = \<Union>iter n f ` X"
+  hence ind_hyp2: "iter n f (\<Union>X) = \<Union>iter n f ` X"
+    by auto
+  have "iter (Suc n) f (\<Union>X) = f (iter n f (\<Union> X))"
+    by simp
+  also have "... = f (\<Union>iter n f ` X)"
+    by (metis ind_hyp2)
+  also have "... = \<Union>f ` iter n f ` X"
+    by (metis f_jp)
+  also have "... = \<Union>iter (Suc n) f ` X"
+    by (auto simp add: image_def)
+  finally show "iter (Suc n) f (\<Union>X) = \<Union>iter (Suc n) f ` X" .
+qed
+
+lemma eval_jp: "eval_skat_expr D s (\<Union>X) = \<Union>(eval_skat_expr D s ` X)"
+proof (induct s arbitrary: X)
+  fix x and s :: "'b wf_trm" and X
+  show "eval_skat_expr D (SKLeaf x s) (\<Union>X) = \<Union>eval_skat_expr D (SKLeaf x s) ` X"
+    by (auto simp add: wf_assigns_def set_mems_def)
+next
+  fix s t :: "'b skat_expr" and X
+  assume "\<And>X. eval_skat_expr D s (\<Union>X) = \<Union>eval_skat_expr D s ` X"
+  and "\<And>X. eval_skat_expr D t (\<Union>X) = \<Union>eval_skat_expr D t ` X"
+  thus "eval_skat_expr D (s :\<oplus>: t) (\<Union>X) = \<Union>eval_skat_expr D (s :\<oplus>: t) ` X"
+    by auto
+next
+  fix s t :: "'b skat_expr" and X
+  assume asm1: "\<And>X. eval_skat_expr D s (\<Union>X) = \<Union>eval_skat_expr D s ` X"
+  and asm2: "\<And>X. eval_skat_expr D t (\<Union>X) = \<Union>eval_skat_expr D t ` X"
+  have "eval_skat_expr D (s :\<odot>: t) (\<Union>X) = eval_skat_expr D t (eval_skat_expr D s (\<Union>X))"
+    by simp
+  also have "... = eval_skat_expr D t (\<Union>eval_skat_expr D s ` X)"
+    by (simp add: asm1[of X])
+  also have "... = \<Union>(eval_skat_expr D t ` eval_skat_expr D s ` X)"
+    by (insert asm2[of "eval_skat_expr D s ` X"])
+  also have "... = \<Union>eval_skat_expr D (s :\<odot>: t) ` X"
+    by simp
+  finally show "eval_skat_expr D (s :\<odot>: t) (\<Union>X) = \<Union>eval_skat_expr D (s :\<odot>: t) ` X" .
+next
+  fix s :: "'b skat_expr" and X
+  assume asm: "\<And>X. eval_skat_expr D s (\<Union>X) = \<Union>eval_skat_expr D s ` X"
+  show "eval_skat_expr D (SKStar s) (\<Union>X) = \<Union>eval_skat_expr D (SKStar s) ` X"
+  proof auto
+    fix x n assume "x \<in> iter n (eval_skat_expr D s) (\<Union>X)"
+    hence "x \<in> \<Union>(iter n (eval_skat_expr D s) ` X)"
+      by (metis asm iter_jp)
+    thus "\<exists>y\<in>X. \<exists>n. x \<in> iter n (eval_skat_expr D s) y"
+      by (metis (no_types) UnionE image_iff)
+  next
+    fix x y n assume "y \<in> X" and "x \<in> iter n (eval_skat_expr D s) y"
+    hence "\<exists>n. x \<in> \<Union>(iter n (eval_skat_expr D s) ` X)"
+      by (metis UnionI image_eqI)
+    thus "\<exists>n. x \<in> iter n (eval_skat_expr D s) (\<Union>X)"
+      by (metis asm iter_jp)
+  qed
+next
+  fix P :: "'b wf_pred bexpr" and X
+  show "eval_skat_expr D (SKBool P) (\<Union>X) = \<Union>eval_skat_expr D (SKBool P) ` X"
+    by (auto simp add: filter_set_def)
+next
+  fix X
+  show "eval_skat_expr D SKOne (\<Union>X) = \<Union>eval_skat_expr D SKOne ` X"
+    by auto
+next
+  fix X
+  show "eval_skat_expr D SKZero (\<Union>X) = \<Union>eval_skat_expr D SKZero ` X"
+    by auto
+qed
+
+lemma eval_star_slide:
+  fixes \<Delta> :: "'b mems"
+  shows "eval_skat_expr D (SKStar x :\<odot>: x) \<Delta> = eval_skat_expr D (x :\<odot>: SKStar x) \<Delta>"
+  apply (simp add: eval_star_power del: eval_skat_expr.simps(5))
+  apply (simp add: eval_jp)
+  apply auto
+  apply (metis (no_types) iter.simps(2) eval_iter eval_power_def)
+  by (metis (no_types) iter.simps(2) eval_iter eval_power_def)
+
+lemma eval_star_unfoldr:
+  fixes \<Delta> :: "'b mems"
+  shows "eval_skat_expr D (SKOne :\<oplus>: SKStar x :\<odot>: x :\<oplus>: SKStar x) \<Delta> = eval_skat_expr D (SKStar x) \<Delta>"
+  by (subst eval_star_unfoldl[symmetric], insert eval_star_slide, auto)
+
+lemma eval_star_inductl:
+  assumes asm2: "\<forall>\<Delta>::'b mems. eval_skat_expr D (z :\<oplus>: x :\<odot>: y :\<oplus>: y) \<Delta> = eval_skat_expr D y \<Delta>"
+  shows "\<forall>\<Delta>. eval_skat_expr D (SKStar x :\<odot>: z :\<oplus>: y) \<Delta> = eval_skat_expr D y \<Delta>"
+proof (auto simp add: eval_star_power eval_jp eval_power_def simp del: eval_skat_expr.simps(5))
+  fix \<Delta> :: "'b mems" and mem :: "'b mem" and n
+  assume "mem \<in> eval_skat_expr D z (iter n (eval_skat_expr D x) \<Delta>)"
+  hence "mem \<in> eval_skat_expr D (z :\<oplus>: x :\<odot>: y :\<oplus>: y) \<Delta>"
+  proof (induct n arbitrary: \<Delta>, simp, simp only: iter.simps eval_iter1)
+    fix m and \<Gamma> :: "'b mems"
+    assume "\<And>\<Delta>. mem \<in> eval_skat_expr D z (iter m (eval_skat_expr D x) \<Delta>) \<Longrightarrow>
+                mem \<in> eval_skat_expr D (z :\<oplus>: x :\<odot>: y :\<oplus>: y) \<Delta>"
+      and "mem \<in> eval_skat_expr D z (iter m (eval_skat_expr D x) (eval_skat_expr D x \<Gamma>))"
+    hence a: "mem \<in> eval_skat_expr D (z :\<oplus>: x :\<odot>: y :\<oplus>: y) (eval_skat_expr D x \<Gamma>)"
+      by auto
+    thus "mem \<in> eval_skat_expr D (z :\<oplus>: x :\<odot>: y :\<oplus>: y) \<Gamma>"
+      by (auto, (metis a asm2)+)
+  qed
+  thus "mem \<in> eval_skat_expr D y \<Delta>"
+    by (metis asm2)
+qed
+
+lemma eval_iso2:
+  assumes "\<And>mem. mem \<in> \<Delta> \<Longrightarrow> mem \<in> \<Gamma>"
+  and "mem \<in> eval_skat_expr D s \<Delta>"
+  shows "mem \<in> eval_skat_expr D s \<Gamma>"
+proof -
+  have "\<Delta> \<subseteq> \<Gamma>"
+    by (insert assms(1), auto)
+  thus ?thesis
+    by (metis assms(2) eval_iso set_mp)
+qed
+
+lemma eval_star_inductr:
+  assumes asm2: "\<forall>\<Delta>::'b mems. eval_skat_expr D (z :\<oplus>: y :\<odot>: x :\<oplus>: y) \<Delta> = eval_skat_expr D y \<Delta>"
+  shows "\<forall>\<Delta>. eval_skat_expr D (z :\<odot>: SKStar x :\<oplus>: y) \<Delta> = eval_skat_expr D y \<Delta>"
+proof auto
+  fix \<Delta> :: "'b mems" and mem :: "'b mem" and n
+  assume "mem \<in> iter n (eval_skat_expr D x) (eval_skat_expr D z \<Delta>)"
+  hence "mem \<in> eval_skat_expr D (z :\<oplus>: y :\<odot>: x :\<oplus>: y) \<Delta>"
+  proof (induct n arbitrary: mem, simp)
+    fix n mem
+    assume asm:
+      "\<And>mem. mem \<in> iter n (eval_skat_expr D x) (eval_skat_expr D z \<Delta>) \<Longrightarrow>
+             mem \<in> eval_skat_expr D (z :\<oplus>: y :\<odot>: x :\<oplus>: y) \<Delta>"
+    and "mem \<in> iter (Suc n) (eval_skat_expr D x) (eval_skat_expr D z \<Delta>)"
+    hence "mem \<in> eval_skat_expr D x (iter n (eval_skat_expr D x) (eval_skat_expr D z \<Delta>))"
+      by simp
+    hence "mem \<in> eval_skat_expr D x (eval_skat_expr D (z :\<oplus>: y :\<odot>: x :\<oplus>: y) \<Delta>)"
+      by (smt asm eval_iso2)
+    thus "mem \<in> eval_skat_expr D (z :\<oplus>: y :\<odot>: x :\<oplus>: y) \<Delta>"
+      by (metis (lifting) UnI1 UnI2 asm2 eval_skat_expr.simps(3) eval_skat_expr.simps(4))
+  qed
+  thus "mem \<in> eval_skat_expr D y \<Delta>"
+    by (metis asm2)
 qed
 
 theorem hunt_con_eval: "hunt_con s t \<Longrightarrow> \<forall>\<Delta>. eval_bexpr D s \<Delta> = eval_bexpr D t \<Delta>"
@@ -167,29 +334,30 @@ next
   fix x show "\<forall>\<Delta>. eval_skat_expr D (SKZero :\<odot>: x) \<Delta> = eval_skat_expr D SKZero \<Delta>"
     by (simp, metis eval_mod1)
 next
-  fix x show "\<forall>\<Delta>. eval_skat_expr D (SKOne :\<oplus>: x :\<odot>: SKStar x :\<oplus>: SKStar x) \<Delta> = eval_skat_expr D (SKStar x) \<Delta>"
-    sorry (* unfolding *)
+  fix x
+  show "\<forall>\<Delta>. eval_skat_expr D (SKOne :\<oplus>: x :\<odot>: SKStar x :\<oplus>: SKStar x) \<Delta> = eval_skat_expr D (SKStar x) \<Delta>"
+    by (metis eval_star_unfoldl)
 next
-  fix x show "\<forall>\<Delta>. eval_skat_expr D (SKOne :\<oplus>: SKStar x :\<odot>: x :\<oplus>: SKStar x) \<Delta> = eval_skat_expr D (SKStar x) \<Delta>"
-    sorry
+  fix x
+  show "\<forall>\<Delta>. eval_skat_expr D (SKOne :\<oplus>: SKStar x :\<odot>: x :\<oplus>: SKStar x) \<Delta> = eval_skat_expr D (SKStar x) \<Delta>"
+    by (metis eval_star_unfoldr)
 next
-  fix z x y assume "skat_con (z :\<oplus>: x :\<odot>: y :\<oplus>: y) y"
-  and "\<forall>\<Delta>. eval_skat_expr D (z :\<oplus>: x :\<odot>: y :\<oplus>: y) \<Delta> = eval_skat_expr D y \<Delta>"
+  fix z x y assume "\<forall>\<Delta>. eval_skat_expr D (z :\<oplus>: x :\<odot>: y :\<oplus>: y) \<Delta> = eval_skat_expr D y \<Delta>"
   thus "\<forall>\<Delta>. eval_skat_expr D (SKStar x :\<odot>: z :\<oplus>: y) \<Delta> = eval_skat_expr D y \<Delta>"
-    sorry
+    by (metis eval_star_inductl)
 next
- fix z y x assume "skat_con (z :\<oplus>: y :\<odot>: x :\<oplus>: y) y"
- and "\<forall>\<Delta>. eval_skat_expr D (z :\<oplus>: y :\<odot>: x :\<oplus>: y) \<Delta> = eval_skat_expr D y \<Delta>"
- thus "\<forall>\<Delta>. eval_skat_expr D (z :\<odot>: SKStar x :\<oplus>: y) \<Delta> = eval_skat_expr D y \<Delta>"
-   sorry
+  fix z y x assume "skat_con (z :\<oplus>: y :\<odot>: x :\<oplus>: y) y"
+  and "\<forall>\<Delta>. eval_skat_expr D (z :\<oplus>: y :\<odot>: x :\<oplus>: y) \<Delta> = eval_skat_expr D y \<Delta>"
+  thus "\<forall>\<Delta>. eval_skat_expr D (z :\<odot>: SKStar x :\<oplus>: y) \<Delta> = eval_skat_expr D y \<Delta>"
+    by (metis eval_star_inductr)
 next
- fix x y :: "'a wf_pred bexpr" assume "hunt_con x y"
- hence "\<forall>\<Delta>. eval_bexpr D x \<Delta> = eval_bexpr D y \<Delta>"
-   by (metis hunt_con_eval)
- hence "eval_bexpr D x = eval_bexpr D y"
-   by auto
- thus "\<forall>\<Delta>. eval_skat_expr D (SKBool x) \<Delta> = eval_skat_expr D (SKBool y) \<Delta>"
-   by (simp del: filter_set_def)
+  fix x y :: "'a wf_pred bexpr" assume "hunt_con x y"
+  hence "\<forall>\<Delta>. eval_bexpr D x \<Delta> = eval_bexpr D y \<Delta>"
+    by (metis hunt_con_eval)
+  hence "eval_bexpr D x = eval_bexpr D y"
+    by auto
+  thus "\<forall>\<Delta>. eval_skat_expr D (SKBool x) \<Delta> = eval_skat_expr D (SKBool y) \<Delta>"
+    by (simp del: filter_set_def)
 next
   fix x y show "\<forall>\<Delta>. eval_skat_expr D (SKBool (x :\<cdot>: y)) \<Delta> = eval_skat_expr D (SKBool x :\<odot>: SKBool y) \<Delta>"
     by (auto, (metis empty_iff singleton_iff)+)
@@ -197,74 +365,181 @@ next
   fix x y show "\<forall>\<Delta>. eval_skat_expr D (SKBool (x :+: y)) \<Delta> = eval_skat_expr D (SKBool x :\<oplus>: SKBool y) \<Delta>"
     by (auto, (metis empty_iff singleton_iff)+)
 next
-  fix Y and s :: "'a wf_trm" and X and t :: "'a wf_trm" assume Ys: "Y \<inter> FV s = {}"
-  thus "\<forall>\<Delta>. eval_skat_expr D (SKLeaf X s :\<odot>: SKLeaf Y t) \<Delta> =
-            eval_skat_expr D (SKLeaf Y (t[X|s]) :\<odot>: SKLeaf X s) \<Delta>"
-  proof (intro allI)
-    fix \<Delta>
-    have "eval_skat_expr D (SKLeaf X s :\<odot>: SKLeaf Y t) \<Delta> =
-          eval_skat_expr D (SKLeaf Y t) (eval_skat_expr D (SKLeaf X s) \<Delta>)"
-      by simp
-    also have "... = eval_skat_expr D (SKLeaf X s) (eval_skat_expr D (SKLeaf Y (t[X|s])) \<Delta>)"
-      sorry
-    also have "... = eval_skat_expr D (SKLeaf Y (t[X|s]) :\<odot>: SKLeaf X s) \<Delta>"
-      by simp
-    finally show "eval_skat_expr D (SKLeaf X s :\<odot>: SKLeaf Y t) \<Delta> =
-                  eval_skat_expr D (SKLeaf Y (t[X|s]) :\<odot>: SKLeaf X s) \<Delta>" .
-  qed
+  fix x y :: nat and s t :: "'a wf_trm" assume "x \<noteq> y" and "y \<notin> FV s"
+  thus "\<forall>\<Delta>. eval_skat_expr D (SKLeaf x s :\<odot>: SKLeaf y t) \<Delta> =
+            eval_skat_expr D (SKLeaf y (t[x|s]) :\<odot>: SKLeaf x s) \<Delta>"
+    by (simp, metis eval_wf_assigns1)
 next
-
+  fix x y :: nat and s t :: "'a wf_trm" assume "x \<noteq> y" and "x \<notin> FV s"
+  thus "\<forall>\<Delta>. eval_skat_expr D (SKLeaf x s :\<odot>: SKLeaf y t) \<Delta> =
+            eval_skat_expr D (SKLeaf x s :\<odot>: SKLeaf y (t[x|s])) \<Delta>"
+    by (simp, metis eval_wf_assigns2)
+next
+  fix x s t
+  show "\<forall>\<Delta>. eval_skat_expr D (SKLeaf x s :\<odot>: SKLeaf x t) \<Delta> =
+            eval_skat_expr D (SKLeaf x (t[x|s])) \<Delta>"
+    by (simp, metis eval_wf_assigns3)
+next
+  fix x t \<phi>
+  show "\<forall>\<Delta>. eval_skat_expr D (SKBool (bexpr_map (wf_pred_subst x t) \<phi>) :\<odot>: SKLeaf x t) \<Delta> =
+            eval_skat_expr D (SKLeaf x t :\<odot>: SKBool \<phi>) \<Delta>"
+    sorry
 qed
 
 lift_definition eval ::
-  "('a::ranked_alphabet, 'b) interp \<Rightarrow> 'a skat \<Rightarrow> 'b mem \<Rightarrow> 'b mem"
+  "('a::ranked_alphabet, 'b) interp \<Rightarrow> 'a skat \<Rightarrow> 'b mems \<Rightarrow> 'b mems"
   is eval_skat_expr
 proof -
   fix D :: "('a::ranked_alphabet, 'b) interp" and s t :: "'a skat_expr"
   assume "skat_con s t"
-  hence "\<forall>\<Delta>. eval_skat_expr D s (\<Delta> :: 'b mem) = eval_skat_expr D t \<Delta>"
+  hence "\<forall>\<Delta>. eval_skat_expr D s \<Delta> = eval_skat_expr D t \<Delta>"
     by (metis skat_con_eval)
   thus "eval_skat_expr D s = eval_skat_expr D t"
     by auto
 qed
 
+definition expr_determ ::
+  "('a::ranked_alphabet, 'b) interp \<Rightarrow> 'a skat_expr \<Rightarrow> bool"
+  where
+  "expr_determ D s \<equiv> \<forall>\<Delta>. \<exists>mem. eval_skat_expr D s \<Delta> = {mem}"
+
+fun skat_prog :: "'a::ranked_alphabet prog \<Rightarrow> 'a skat" where
+  "skat_prog (If \<phi> x y) = pred \<phi> \<cdot> skat_prog x + !(pred \<phi>) \<cdot> skat_prog y"
+| "skat_prog (While \<phi> x) = (pred \<phi> \<cdot> skat_prog x)\<^sup>\<star> \<cdot> !(pred \<phi>)"
+| "skat_prog (Seq []) = \<one>"
+| "skat_prog (Seq (x#xs)) = skat_prog x \<cdot> skat_prog (Seq xs)"
+| "skat_prog (Assign x s) = x := s"
+
+fun skat_expr_prog :: "'a::ranked_alphabet prog \<Rightarrow> 'a skat_expr" where
+  "skat_expr_prog (If \<phi> x y) =
+    (SKBool (BLeaf \<phi>) :\<odot>: skat_expr_prog x) :\<oplus>: (SKBool (BNot (BLeaf \<phi>)) :\<odot>: skat_expr_prog y)"
+| "skat_expr_prog (While \<phi> x) = SKStar (SKBool (BLeaf \<phi>) :\<odot>: skat_expr_prog x) :\<odot>: SKBool (BNot (BLeaf \<phi>))"
+| "skat_expr_prog (Seq []) = SKOne"
+| "skat_expr_prog (Seq (x#xs)) = skat_expr_prog x :\<odot>: skat_expr_prog (Seq xs)"
+| "skat_expr_prog (Assign x s) = SKLeaf x s"
+
+lemma "skat_prog pgm = \<lfloor>skat_expr_prog pgm\<rfloor>"
+proof (induct pgm)
+  fix pgms :: "'a prog list"
+  assume "\<forall>pgm\<in>set pgms. skat_prog pgm = \<lfloor>skat_expr_prog pgm\<rfloor>"
+  thus "skat_prog (Seq pgms) = \<lfloor>skat_expr_prog (Seq pgms)\<rfloor>"
+    by (induct pgms, auto)
+qed auto
+
 context valid_interp
 begin
 
-  definition module :: "'a skat \<Rightarrow> 'b mem \<Rightarrow> 'b mem" (infix "\<Colon>" 75) where
-    "module \<equiv> eval D"
+  definition module :: "'b mems \<Rightarrow> 'a skat \<Rightarrow> 'b mems" (infix "\<Colon>" 75) where
+    "module \<Delta> x \<equiv> eval D x \<Delta>"
 
-  definition mod_le :: "'b mem \<Rightarrow> 'b mem \<Rightarrow> bool" (infix "\<preceq>" 60) where
+  definition mod_le :: "'b mems \<Rightarrow> 'b mems \<Rightarrow> bool" (infix "\<preceq>" 60) where
     "x \<preceq> y \<equiv> x \<union> y = y"
-
-  declare module_def [skat_simp]
-  declare mod_le_def [skat_simp]
 
   (* Properties from Kleene modules and linear languages by Hans Leiss *)
 
-  lemma "r \<Colon> {} = {}"
-    by (skat_simp, transfer, metis eval_mod1)
+  lemma mod_empty [simp]: "{} \<Colon> r = {}"
+    by (simp add: module_def, transfer, metis eval_mod1)
 
-  lemma "r \<Colon> (b \<union> a) = r \<Colon> b \<union> r \<Colon> a"
-    by (skat_simp, transfer, metis eval_mod2)
+  lemma "(a \<union> b) \<Colon> r = a \<Colon> r \<union> b \<Colon> r"
+    by (simp add: module_def, transfer, metis eval_mod2)
 
-  lemma "\<zero> \<Colon> a = {}"
-    by (skat_simp, transfer, simp)
+  lemma mod_zero [simp]: "a \<Colon> \<zero> = {}"
+    by (simp add: module_def, transfer, simp)
 
-  lemma "(r + s) \<Colon> a = r \<Colon> a \<union> s \<Colon> a"
-    by (skat_simp, transfer, simp)
+  lemma mod_plus: "a \<Colon> (r + s) = a \<Colon> r \<union> a \<Colon> s"
+    by (simp add: module_def, transfer, simp)
 
-  lemma "\<one> \<Colon> a = a"
-    by (skat_simp, transfer, simp)
+  lemma mod_one [simp]: "a \<Colon> \<one> = a"
+    by (simp add: module_def, transfer, simp)
 
-  (* This is the opposite from the paper -- it has r \<Colon> (s \<Colon> a) *)
-  lemma "(r \<cdot> s) \<Colon> a = s \<Colon> (r \<Colon> a)"
-    by (skat_simp, transfer, simp)
+  lemma mod_mult: "a \<Colon> (r \<cdot> s) = (a \<Colon> r) \<Colon> s"
+    by (simp add: module_def, transfer, simp)
 
-  lemma "r \<Colon> b \<union> a \<preceq> b \<Longrightarrow> r\<^sup>\<star> \<Colon> a \<preceq> b"
-    by (skat_simp, transfer, metis eval_mod3)
+  lemma "a \<union> b \<Colon> r \<preceq> b \<Longrightarrow> a \<Colon> r\<^sup>\<star> \<preceq> b"
+    apply (simp add: module_def mod_le_def)
+    apply transfer
+    by (metis (lifting) eval_mod3 sup.commute)
 
+  lemma mod_assign: "\<Delta> \<Colon> x := s = wf_assigns D x s \<Delta>"
+    apply (simp add: module_def)
+    apply transfer
+    apply simp
+    done
+
+  lemma mod_pred_expr: "\<Delta> \<Colon> pred_expr P = filter_set (eval_bexpr D P) \<Delta>"
+    apply (simp add: module_def)
+    apply transfer
+    apply simp
+    done
+
+  lemma mod_eval: "\<Delta> \<Colon> \<lfloor>s\<rfloor> = eval_skat_expr D s \<Delta>"
+  proof -
+    have "eval_skat_expr D s \<Delta> = \<Delta> \<Colon> abs_skat s"
+      by (simp add: module_def, transfer, auto)
+    thus ?thesis
+      by (metis unfold_is_abs)
+  qed
+
+  lemma mod_star_eval: "\<Delta> \<Colon> \<lfloor>s\<rfloor>\<^sup>\<star> = (\<Union>n. iter n (eval_skat_expr D s) \<Delta>)"
+    by (subgoal_tac "\<lfloor>s\<rfloor>\<^sup>\<star> = \<lfloor>SKStar s\<rfloor>", simp only: mod_eval, transfer, auto)
+
+  definition terminates :: "'a prog \<Rightarrow> bool" where
+    "terminates prgm \<equiv> \<exists>steps. \<forall>mem. eval_prog steps D mem prgm \<noteq> None"
+
+  definition deterministic :: "'a skat \<Rightarrow> bool" where
+    "deterministic s \<equiv> \<forall>mem. card ({mem} \<Colon> s) = 1"
+
+  lemma det_mult: "\<lbrakk>deterministic x; deterministic y\<rbrakk> \<Longrightarrow> deterministic (x \<cdot> y)"
+    by (auto simp add: deterministic_def mod_mult, metis card_eq_SucD)
+
+  lemma "terminates pgm \<Longrightarrow> deterministic (skat_prog pgm)"
+  proof (induct pgm)
+    show "\<forall>x\<in>set[]. deterministic (skat_prog x)"
+      by auto
+  next
+    fix xs assume "\<forall>x\<in>set xs. deterministic (skat_prog x)"
+    thus "deterministic (skat_prog (Seq xs))"
+      by (induct xs, simp add: deterministic_def, auto intro: det_mult)
+  next
+    fix x s
+    show "deterministic (skat_prog (Assign x s))"
+      by (simp add: deterministic_def mod_assign wf_assigns_def set_mems_def)
+  next
+    fix \<phi> pgm1 pgm2
+    assume "deterministic (skat_prog pgm1)"
+    and "deterministic (skat_prog pgm2)"
+    thus "deterministic (skat_prog (If \<phi> pgm1 pgm2))"
+    proof (auto simp add: deterministic_def)
+      fix mem
+      assume "\<forall>mem. card ({mem} \<Colon> skat_prog pgm1) = Suc 0"
+      and "\<forall>mem. card ({mem} \<Colon> skat_prog pgm2) = Suc 0"
+      hence "card ({mem} \<Colon> (pred_expr (BLeaf \<phi>) \<cdot> skat_prog pgm1 +
+                            pred_expr (BNot (BLeaf \<phi>)) \<cdot> skat_prog pgm2)) =
+             Suc 0"
+        by (simp add: mod_plus mod_mult mod_pred_expr)
+      thus "card ({mem} \<Colon> (pred \<phi> \<cdot> skat_prog pgm1 + !(pred \<phi>) \<cdot> skat_prog pgm2)) = Suc 0"
+        by (metis pred_expr_not pred_to_expr)
+    qed
+  next
+    fix \<phi> pgm
+    assume "deterministic (skat_prog pgm)"
+    thus "deterministic (skat_prog (While \<phi> pgm))"
+    proof (auto simp add: deterministic_def mod_mult)
+      fix mem
+      assume "\<forall>mem. card ({mem} \<Colon> skat_prog pgm) = Suc 0"
+      have "card (({mem} \<Colon> \<lfloor>(SKBool (BLeaf \<phi>) :\<odot>: skat_expr_prog pgm)\<rfloor>\<^sup>\<star>) \<Colon> pred_expr (BNot (BLeaf \<phi>))) = Suc 0"
+        apply (simp only: mod_star_eval mod_pred_expr)
+        apply auto
+        apply (simp add: eval_skat_expr.simps)
+        
+      thus "card (({mem} \<Colon> (pred \<phi> \<cdot> skat_prog pgm)\<^sup>\<star>) \<Colon> !(pred \<phi>)) = Suc 0"
+        
+    qed
+  qed
 end
+
+definition deterministic :: "'a::ranked_alphabet skat \<Rightarrow> bool" where
+  "deterministic s \<equiv> \<forall>D. valid_interp D \<longrightarrow> valid_interp.deterministic D s"
 
 end
 
